tests/lean/1814.lean
@@ -1,0 +1,12 @@
+example : ∀ (p q : Prop), p → q → p :=
+begin
+  intros p p h1 h2,
+  exact h2,
+end
+
+example : ∀ (p q : Prop), p → q → p :=
+begin
+  intros p p h1 h2,
+  dedup,
+  exact h2,
+end
